_pages/about.markdown
@@ -3,18 +3,18 @@ title: About
 permalink: /about/
 ---
 
-# Vision
+## Vision
 
 A common, open source, mechanized foundation for computing & mathematics.
 
-# Mission
+## Mission
 
 Widespread adoption of mechanized logic by open source & industry.
 
-# Strategy
+## Strategy
 
 Add value & reduce barriers to entry.
 
-# Get involved
+## Get involved
 
 We love to collaborate! Please reach out 😊
