_pages/blog.markdown
@@ -2,7 +2,8 @@
 title: Blog
 permalink: /blog/
 ---
-<h3 class="archive__subtitle">{{ site.data.ui-text[site.locale].recent_posts | default: "Recent Posts" }}</h3>
+
+## Recent Posts
 
 {% if paginator %}
   {% assign posts = paginator.posts %}
