_pages/projects.markdown
@@ -1,0 +1,6 @@
+---
+title: Projects
+permalink: /projects/
+---
+
+_Coming soon_
