_pages/resources.markdown
@@ -1,0 +1,22 @@
+---
+title: Resources
+permalink: /resources/
+---
+
+## Downloads
+
+* [Coq](https://coq.inria.fr/download)
+
+## Open source libraries
+
+* [Awesome Coq Projects](https://github.com/sindresorhus/awesome#readme)
+* [Recent GitHub Activity](https://github.com/search?o=desc&q=language%3Acoq&s=updated&type=Repositories)
+
+## Books
+
+* [Software Foundations](https://softwarefoundations.cis.upenn.edu/)
+* [Certified Programming with Dependent Types](http://adam.chlipala.net/cpdt/)
+
+## Domain-specific books
+
+* [Formal Reasoning About Programs](http://adam.chlipala.net/frap/)
